candle/prover/compute/computeScript.sml
@@ -38,6 +38,9 @@ Definition compute_thms_def:
     (* BIT1       *) _BIT1 _N === _SUC (_ADD _N _N);
     (* ADD        *) _ADD (_NUMERAL _0) _N === _N;
     (* ADD        *) _ADD (_SUC _M) _N === _SUC (_ADD _M _N);
+    (* SUB        *) _SUB (_NUMERAL _0) _N === _NUMERAL _0;
+    (* SUB        *) _SUB _M (_NUMERAL _0) === _M;
+    (* SUB        *) _SUB (_SUC _M) (_SUC _N) === _SUB _M _N;
     (* CVAL_ADD   *) _CVAL_ADD (_CVAL_NUM _M) (_CVAL_NUM _N) ===
                      _CVAL_NUM (_ADD _M _N);
     (* CVAL_ADD   *) _CVAL_ADD (_CVAL_NUM _M) (_CVAL_PAIR _P1 _Q1) ===
@@ -45,6 +48,14 @@ Definition compute_thms_def:
     (* CVAL_ADD   *) _CVAL_ADD (_CVAL_PAIR _P1 _Q1) (_CVAL_NUM _N) ===
                      _CVAL_NUM _N;
     (* CVAL_ADD   *) _CVAL_ADD (_CVAL_PAIR _P1 _Q1) (_CVAL_PAIR _P2 _Q2) ===
+                     _CVAL_NUM (_NUMERAL _0);
+    (* CVAL_SUB   *) _CVAL_SUB (_CVAL_NUM _M) (_CVAL_NUM _N) ===
+                     _CVAL_NUM (_SUB _M _N);
+    (* CVAL_SUB   *) _CVAL_SUB (_CVAL_NUM _M) (_CVAL_PAIR _P1 _Q1) ===
+                     _CVAL_NUM _M;
+    (* CVAL_SUB   *) _CVAL_SUB (_CVAL_PAIR _P1 _Q1) (_CVAL_NUM _N) ===
+                     _CVAL_NUM _N;
+    (* CVAL_SUB   *) _CVAL_SUB (_CVAL_PAIR _P1 _Q1) (_CVAL_PAIR _P2 _Q2) ===
                      _CVAL_NUM (_NUMERAL _0);
     (* CVAL_IF    *) _CVAL_IF (_CVAL_NUM (_SUC _M)) _P1 _Q1 === _P1;
     (* CVAL_IF    *) _CVAL_IF (_CVAL_PAIR _P2 _Q2) _P1 _Q1 === _P1;
